Ticket lock example

exercises/ticket_lock.v
@@ -61,20 +61,19 @@ Definition release : val :=
   specifications to figure out exactly what needs to be proven.
 *)
 
-Definition RA : cmra
-  (* := insert your definition here *). Admitted.
+Definition RA : cmra := authR (prodUR (optionUR (exclR natO)) (gset_disjR nat)).
 
 Section proofs.
 Context `{!heapGS Σ, !inG Σ RA}.
-Let N := nroot .@ "ticket_lock".
 
+Definition N := nroot .@ "ticket_lock".
 (**
   This time around, we know that the thread is locked by a thread with a
   specific ticket. As such, we first define a predicate [locked_by]
   which states that the lock is locked by ticket [o].
 *)
-Definition locked_by (γ : gname) (o : nat) : iProp Σ
-  (* := insert your definition here *). Admitted.
+
+Definition locked_by (γ : gname) (o : nat) : iProp Σ := own γ (◯ (Excl' o, GSet ∅)).
 
 (** The lock is locked when it has been locked by some ticket. *)
 Definition locked (γ : gname) : iProp Σ :=
@@ -82,19 +81,27 @@ Definition locked (γ : gname) : iProp Σ :=
 
 Lemma locked_excl γ : locked γ -∗ locked γ -∗ False.
 Proof.
-  (* exercise *)
-Admitted.
+  iIntros "[%o Hγ] [%o' Hγ']".
+  rewrite /locked /locked_by.
+  iPoseProof (own_valid_2 with "Hγ Hγ'") as "%Hvalid".
+  rewrite auth_frag_valid pair_valid in Hvalid.
+  destruct Hvalid as [[] _].
+Qed.
 
 (**
   We will also have a predicate signifying that ticket [x] has been
   _issued_. A thread will need to have been issued ticket [x] in order
   to wait for the first counter to become [x].
 *)
-Definition issued (γ : gname) (x : nat) : iProp Σ
-  (* := insert your definition here *). Admitted.
+Definition issued (γ : gname) (x : nat) : iProp Σ :=
+  own γ (◯ (ε, GSet {[ x ]})).
 
-Definition lock_inv (γ : gname) (lo ln : loc) (P : iProp Σ) : iProp Σ
-  (* := insert your definition here *). Admitted.
+Definition lock_inv (γ : gname) (lₒ lₙ : loc) (P : iProp Σ) : iProp Σ :=
+  ∃ o n : nat, 
+    lₒ ↦ #o ∗ 
+    lₙ ↦ #n ∗ 
+    own γ (● (Excl' o, GSet (set_seq 0 n))) ∗
+    ((locked_by γ o ∗ P) ∨ issued γ o).
 
 Definition is_lock (γ : gname) (l : val) (P : iProp Σ) : iProp Σ :=
   ∃ lo ln : loc, ⌜l = (#lo, #ln)%V⌝ ∗ inv N (lock_inv γ lo ln P).
@@ -105,26 +112,172 @@ Definition is_lock (γ : gname) (l : val) (P : iProp Σ) : iProp Σ :=
 Lemma mk_lock_spec P :
   {{{ P }}} mk_lock #() {{{ γ l, RET l; is_lock γ l P }}}.
 Proof.
-  (* exercise *)
-Admitted.
+  iIntros (Φ) "HP HΦ".
+  rewrite /mk_lock.
+  wp_pures.
+  wp_alloc lₒ as "Hlₒ".
+  wp_alloc lₙ as "Hlₙ".
+  wp_pures.
+  iMod (own_alloc (● (Excl' 0, GSet ∅) ⋅ ◯ (Excl' 0, GSet ∅))) as "(%γ & Hγ & Ho)".
+  { by apply auth_both_valid_discrete. }
+  iApply "HΦ".
+  rewrite /is_lock.
+  iExists lₙ, lₒ.
+  iSplitR; first done.
+  iApply inv_alloc.
+  rewrite /lock_inv.
+  iExists 0, 0.
+  iFrame.
+  iLeft.
+  iFrame.
+Qed.
 
 Lemma wait_spec γ l P x :
   {{{ is_lock γ l P ∗ issued γ x }}}
     wait #x l
   {{{ RET #(); locked γ ∗ P }}}.
 Proof.
-  (* exercise *)
-Admitted.
+  iIntros (Φ) "((%lₒ & %lₙ & -> & #Hinv) & Hissued) HΦ".
+  iLöb as "IH".
+  wp_rec.
+  wp_pures.
+  wp_bind (! _)%E.
+  iInv "Hinv" as "(%o & %n & Hlₒ & Hlₙ & Hγ & Hlock)".
+  wp_load.
+  destruct (decide (o = x)).
+  - subst. iDestruct "Hlock" as "[[Hlock HP] | H]".
+    * iFrame.
+      iModIntro.
+      wp_pures.
+      rewrite -> bool_decide_eq_true_2 by done.
+      wp_pures.
+      iApply "HΦ".
+      by iFrame.
+    * rewrite /issued.
+      iPoseProof (own_valid_2 with "Hissued H") as "%H".
+      rewrite auth_frag_valid /= in H.
+      rewrite pair_valid /= in H.
+      set_solver.
+  - iFrame.
+    iModIntro.
+    wp_pures.
+    rewrite -> bool_decide_eq_false_2 by (intros Heq; simplify_eq).
+    wp_pures.
+    by iApply ("IH" with "Hissued").
+Qed.
 
 Lemma acquire_spec γ l P :
   {{{ is_lock γ l P }}} acquire l {{{ RET #(); locked γ ∗ P }}}.
 Proof.
-  (* exercise *)
-Admitted.
+  iIntros (Φ) "(%lₒ & %lₙ & -> & #Hinv) HΦ".
+  iLöb as "IH".
+  wp_rec.
+  wp_pures.
+  wp_bind (! _)%E.
+  iInv "Hinv" as "(%o & %n & Hlₒ & Hlₙ & Hγ & Hlock)".
+  wp_load.
+  iSplitL "Hlₒ Hlₙ Hγ Hlock".
+  { by iFrame. }
+  iModIntro.
+  wp_pures.
+  wp_bind (CmpXchg _ _ _).
+  clear o.
+  iInv "Hinv" as "(%o & %n' & Hlₒ & Hlₙ & Hγ & Hlock)".
+  (* Case on whether ticket was dispensed *)
+  destruct (decide (n' = n)).
+  + subst.
+    wp_cmpxchg_suc.
+    replace (Z.of_nat n + 1)%Z with (Z.of_nat (S n)) by lia.
+    (* Frame preserving update; add ticket dispensed to waiting queue *)
+    iMod (own_update _ _ (● (Excl' o, GSet (set_seq 0 (S n))) ⋅ ◯ (ε, GSet {[n]})) with "Hγ") as "[●Hγ ◯Hγ]".
+    { apply auth_update_alloc.
+      apply prod_local_update_2.
+      rewrite set_seq_S_end_union_L.
+      rewrite -gset_disj_union.
+      2: { apply set_seq_S_end_disjoint. }
+      rewrite -{2}(ucmra_unit_right_id (GSet {[n]})).
+      apply gset_disj_alloc_op_local_update.
+      apply (set_seq_S_end_disjoint 0). }
+      iSplitR "HΦ ◯Hγ".
+      - rewrite /lock_inv.
+        iExists o, (S n).
+        by iFrame.
+      - iModIntro.
+        wp_pures.
+        wp_apply (wait_spec with "[Hinv $◯Hγ]").
+        { iExists lₒ, lₙ. by iSplit. }
+        iApply "HΦ".
+    + wp_cmpxchg_fail.
+      { intros Heq. simplify_eq. }
+      iSplitR "HΦ".
+      * by iFrame.
+      * iModIntro.
+        wp_pures.
+        by wp_apply "IH".
+Qed.
 
 Lemma release_spec γ l P :
   {{{ is_lock γ l P ∗ locked γ ∗ P }}} release l {{{ RET #(); True }}}.
 Proof.
+  iIntros (Φ) "((%lₒ & %lₙ & -> & #Hinv) & [%o Hlocked] & HP) HΦ".
+  rewrite /release.
+  wp_pures.
+  wp_bind (! _)%E.
+  iInv "Hinv" as "(%o' & %n & Hlₒ & Hlₙ & ●Hγ & [[>Hlocked' _] | Hissued])".
+  {
+    iExFalso.
+    iApply (locked_excl with "[$Hlocked]").
+    iFrame.
+  }
+  wp_load.
+  iSplitL "Hlₒ Hlₙ Hissued ●Hγ".
+  { rewrite /lock_inv. iExists o', n. by iFrame. }
+  iModIntro.
+  wp_pures.
+  iInv "Hinv" as "(%o'' & %n' & Hlₒ' & Hlₙ' & ●Hγ' & [[>Hlocked' _] | Hissued'])".
+  {
+    iExFalso.
+    iApply (locked_excl with "[$Hlocked]").
+    iFrame.
+  }
+  wp_store.
+  iPoseProof (own_valid_2 with "●Hγ' Hlocked") as "%Hvalid".
+  rewrite auth_both_valid_discrete /= in Hvalid.
+  rewrite pair_included in Hvalid.
+  rewrite Excl_included in Hvalid.
+  destruct Hvalid as [[H _] _].
+  destruct H.
+  iSplitR "HΦ".
+  - replace (Z.of_nat o' + 1)%Z with (Z.of_nat (S o')) by lia.
+    iCombine "●Hγ' Hlocked" as "Hγ".
+   iMod (own_update _ _ (● (Excl' (S o), GSet (set_seq 0 n)) ⋅ ◯ (Excl' (S o), ε)) with "Hγ") as "[Hγ Hexcl]".
+   { apply auth_update. }
+
+  - by iApply "HΦ".
+  { admit. }
+  iNext.
+  (* Frame preserving update; remove ticket from waiting queue *)
+
+  rewrite /issued.
+  iMod (own_update _ _ (● (Excl' o'', GSet ∅) ⋅ ◯ (Excl' o'', GSet ∅)) with "Hγ") as "[●Hγ ◯Hγ]".
+  { }
+  iSplitL "Hlₒ Hlₙ Hlocked' Hγ HP".
+
+    iAssert (locked γ) as "Hl". iSplitL "Hlo".
+    { rewrite /locked. iExists o. iFrame. }
+    iApply locked_excl.
+    iApply (locked_excl with "[$o Hlocked] [$o' Hlo]").
+   rewrite /locked_by.
+   iPoseProof (own_valid_2 with "Hlo Hlocked") as "%H".
+   rewrite auth_frag_valid /= in H.
+   rewrite pair_valid /= in H.
+   destruct H as [[] _].
+  }
+  
+
+  wp_load.
+  iSplitL "Hlₒ Hlₙ".
+  + iFrame. admit. 
   (* exercise *)
 Admitted.
 
